theories/eris/tutorial/readme.md
@@ -55,11 +55,10 @@ You should now be able to build the development by using `dune build`, or `dune 
 
 The tutorial will feature a mix of lectures from the organizers and exercises. The plan is to progress as follows.
 
-1. [logic.v](./logic.v): background on (separation) logic in Rocq.
+1. [basic.v](./basic.v): basic separation logic; "error credits" as separation logic resource; manipulating error credits; simple random sampling.
 2. [quicksort.v](./quicksort.v): correctness of randomized quicksort.
-3. [basic.v](./basic.v): "error credits" as separation logic resource; manipulating error credits; simple random sampling.
-4. [geometric.v](./geometric.v): sampling from the geometric distribution.
-5. [hash_interface.v](./hash_interface.v), [bloom_filter_single.v](./bloom_filter_single.v): Bloom filters based on hash functions. Bound on probability of false positives.
+3. [geometric.v](./geometric.v): sampling from the geometric distribution.
+4. [hash_interface.v](./hash_interface.v), [bloom_filter_single.v](./bloom_filter_single.v): Bloom filters based on hash functions. Bound on probability of false positives.
 
 
 # Contact information
